Weidenbach_Book/CDCL_Two_Watched_Literals_VMTF.thy
@@ -2100,6 +2100,28 @@ lemma abs_l_vmtf_unset_vmtf_dump_unset:
      (auto simp: vmtf_imp_append_remove_iff)
 
 
+lemma vmtf_imp_insert_sort_nth_code_preD:
+  assumes vmtf: \<open>vm \<in> vmtf_imp M\<close>
+  shows \<open>\<forall>x\<in>set (snd vm). x < length (fst (fst vm))\<close>
+proof -
+  obtain A m lst next_search remove where
+    vm: \<open>vm = ((A, m, lst, next_search), remove)\<close>
+    by (cases vm) auto
+
+  obtain xs' ys' where
+    l_vmtf: \<open>l_vmtf (ys' @ xs') m A\<close> and
+    lst: \<open>lst = option_hd (ys' @ xs')\<close> and
+    next_search: \<open>next_search = option_hd xs'\<close> and
+    abs_vmtf: \<open>abs_l_vmtf_remove_inv M ((set xs', set ys'), set remove)\<close> and
+    notin: \<open>l_vmtf_notin (ys' @ xs') m A\<close> and
+    atm_A: \<open>\<forall>L\<in>atms_of \<L>\<^sub>a\<^sub>l\<^sub>l. L < length A\<close> and
+    \<open>\<forall>L\<in>set (ys' @ xs'). L \<in> atms_of \<L>\<^sub>a\<^sub>l\<^sub>l\<close>
+    using vmtf unfolding vmtf_imp_def vm by fast
+  show ?thesis
+    using atm_A abs_vmtf unfolding abs_l_vmtf_remove_inv_def
+    by (auto simp: vm)
+qed
+
 end
 
 
@@ -2207,4 +2229,242 @@ text \<open>Save opposite of the phase (e.g. for literals in the conflict clause
 definition  (in twl_array_code_ops) save_phase_inv :: \<open>nat literal \<Rightarrow> phase_saver \<Rightarrow> phase_saver\<close> where
   \<open>save_phase_inv L \<phi> = \<phi>[atm_of L := \<not>is_pos L]\<close>
 
+
+type_synonym vmtf_assn = \<open>uint32 al_vmtf_atm array \<times> nat \<times> uint32 option \<times> uint32 option\<close>
+type_synonym vmtf_remove_assn = \<open>vmtf_assn \<times> uint32 array_list\<close>
+
+type_synonym phase_saver_assn = \<open>bool array\<close>
+
+instance al_vmtf_atm :: (heap) heap
+proof intro_classes
+  let ?to_pair = \<open>\<lambda>x::'a al_vmtf_atm. (stamp x, get_prev x, get_next x)\<close>
+  have inj': \<open>inj ?to_pair\<close>
+    unfolding inj_def by (intro allI) (case_tac x; case_tac y; auto)
+  obtain to_nat :: \<open>nat \<times> 'a option \<times> 'a option \<Rightarrow> nat\<close> where
+    \<open>inj to_nat\<close>
+    by blast
+  then have \<open>inj (to_nat o ?to_pair)\<close>
+    using inj' by (blast intro: inj_comp)
+  then show \<open>\<exists>to_nat :: 'a al_vmtf_atm \<Rightarrow> nat. inj to_nat\<close>
+    by blast
+qed
+
+
+definition l_vmtf_atm_rel where
+\<open>l_vmtf_atm_rel = {(a', a). stamp a = stamp a' \<and>
+   (get_prev a', get_prev a) \<in> \<langle>uint32_nat_rel\<rangle>option_rel \<and>
+   (get_next a', get_next a) \<in> \<langle>uint32_nat_rel\<rangle>option_rel}\<close>
+
+abbreviation l_vmtf_atm_assn where
+\<open>l_vmtf_atm_assn \<equiv> pure l_vmtf_atm_rel\<close>
+
+lemma l_vmtf_ATM_ref[sepref_fr_rules]:
+  \<open>(uncurry2 (return ooo l_vmtf_ATM), uncurry2 (RETURN ooo l_vmtf_ATM)) \<in>
+    nat_assn\<^sup>k *\<^sub>a (option_assn uint32_nat_assn)\<^sup>k *\<^sub>a (option_assn uint32_nat_assn)\<^sup>k \<rightarrow>\<^sub>a
+    l_vmtf_atm_assn\<close>
+  by sepref_to_hoare
+   (sep_auto simp: l_vmtf_atm_rel_def uint32_nat_rel_def br_def option_assn_alt_def
+     split: option.splits)
+
+lemma stamp_ref[sepref_fr_rules]: \<open>(return o stamp, RETURN o stamp) \<in> l_vmtf_atm_assn\<^sup>k \<rightarrow>\<^sub>a nat_assn\<close>
+  by sepref_to_hoare
+    (auto simp: ex_assn_move_out(2)[symmetric] return_cons_rule ent_ex_up_swap l_vmtf_atm_rel_def
+      simp del: ex_assn_move_out)
+
+lemma get_next_ref[sepref_fr_rules]: \<open>(return o get_next, RETURN o get_next) \<in> l_vmtf_atm_assn\<^sup>k \<rightarrow>\<^sub>a
+   option_assn uint32_nat_assn\<close>
+  unfolding option_assn_pure_conv
+  by sepref_to_hoare (sep_auto simp: return_cons_rule l_vmtf_atm_rel_def)
+
+lemma get_prev_ref[sepref_fr_rules]: \<open>(return o get_prev, RETURN o get_prev) \<in> l_vmtf_atm_assn\<^sup>k \<rightarrow>\<^sub>a
+   option_assn uint32_nat_assn\<close>
+  unfolding option_assn_pure_conv
+  by sepref_to_hoare (sep_auto simp: return_cons_rule l_vmtf_atm_rel_def)
+
+abbreviation vmtf_conc where
+  \<open>vmtf_conc \<equiv> (array_assn l_vmtf_atm_assn *assn nat_assn *assn option_assn uint32_nat_assn
+    *assn option_assn uint32_nat_assn)\<close>
+
+
+abbreviation vmtf_remove_conc :: \<open>vmtf_remove_int \<Rightarrow> vmtf_remove_assn \<Rightarrow> assn\<close> where
+  \<open>vmtf_remove_conc \<equiv> vmtf_conc *assn arl_assn uint32_nat_assn\<close>
+
+definition update_next_search where
+  \<open>update_next_search L = (\<lambda>((A, m, lst, next_search), removed). ((A, m, lst, L), removed))\<close>
+
+lemma update_next_search_ref[sepref_fr_rules]:
+  \<open>(uncurry (return oo update_next_search), uncurry (RETURN oo update_next_search)) \<in>
+      (option_assn uint32_nat_assn)\<^sup>k *\<^sub>a vmtf_remove_conc\<^sup>d \<rightarrow>\<^sub>a vmtf_remove_conc\<close>
+  unfolding option_assn_pure_conv
+  by sepref_to_hoare (sep_auto simp: update_next_search_def)
+
+sepref_definition (in -)l_vmtf_dequeue_code
+   is \<open>uncurry (RETURN oo l_vmtf_dequeue)\<close>
+   :: \<open>[vmtf_dequeue_pre]\<^sub>a
+        uint32_nat_assn\<^sup>k *\<^sub>a (array_assn l_vmtf_atm_assn)\<^sup>d \<rightarrow> array_assn l_vmtf_atm_assn\<close>
+  supply [[goals_limit = 1]]
+  supply option.splits[split]
+  unfolding l_vmtf_dequeue_def vmtf_dequeue_pre_alt_def
+  by sepref
+
+declare l_vmtf_dequeue_code.refine[sepref_fr_rules]
+
+sepref_definition vmtf_dequeue_code
+   is \<open>uncurry (RETURN oo vmtf_dequeue)\<close>
+   :: \<open>[\<lambda>(L,(A,m,lst,next_search)). L < length A \<and> vmtf_dequeue_pre (L, A)]\<^sub>a
+        uint32_nat_assn\<^sup>k *\<^sub>a vmtf_conc\<^sup>d \<rightarrow> vmtf_conc\<close>
+  supply [[goals_limit = 1]]
+  unfolding vmtf_dequeue_def
+  by sepref
+
+declare vmtf_dequeue_code.refine[sepref_fr_rules]
+
+sepref_definition vmtf_enqueue_code
+   is \<open>uncurry (RETURN oo vmtf_enqueue)\<close>
+   :: \<open>[\<lambda>(L,(A,m,lst,next_search)). L < length A \<and> (lst \<noteq> None \<longrightarrow> the lst < length A)]\<^sub>a
+        uint32_nat_assn\<^sup>k *\<^sub>a vmtf_conc\<^sup>d \<rightarrow> vmtf_conc\<close>
+  supply [[goals_limit = 1]]
+  unfolding vmtf_enqueue_def
+  by sepref
+
+declare vmtf_enqueue_code.refine[sepref_fr_rules]
+
+definition insert_sort_inner_nth where
+  \<open>insert_sort_inner_nth A = insert_sort_inner (\<lambda>remove n. stamp (A ! (remove ! n)))\<close>
+
+definition insert_sort_nth where
+  \<open>insert_sort_nth = (\<lambda>(A, _). insert_sort (\<lambda>remove n. stamp (A ! (remove ! n))))\<close>
+
+
+lemma insert_sort_inner_nth_code_helper:
+  assumes \<open>\<forall>x\<in>set ba. x < length a\<close>  and
+      \<open>b < length ba\<close> and
+     mset: \<open>mset ba = mset a2'\<close>  and
+      \<open>a1' < length a2'\<close>
+  shows \<open>a2' ! b < length a\<close>
+  using nth_mem[of b a2'] mset_eq_setD[OF mset] mset_eq_length[OF mset] assms
+  by (auto simp del: nth_mem)
+
+sepref_definition (in -) insert_sort_inner_nth_code
+   is \<open>uncurry2 insert_sort_inner_nth\<close>
+   :: \<open>[\<lambda>((xs, remove), n). (\<forall>x\<in>#mset remove. x < length xs) \<and> n < length remove]\<^sub>a
+  (array_assn l_vmtf_atm_assn)\<^sup>k *\<^sub>a (arl_assn uint32_nat_assn)\<^sup>d *\<^sub>a nat_assn\<^sup>k \<rightarrow>
+  arl_assn uint32_nat_assn\<close>
+  unfolding insert_sort_inner_nth_def insert_sort_inner_def
+  supply [[goals_limit = 1]]
+  supply mset_eq_setD[dest] mset_eq_length[dest]  insert_sort_inner_nth_code_helper[intro]
+  by sepref
+
+declare insert_sort_inner_nth_code.refine[sepref_fr_rules]
+
+sepref_definition (in -) insert_sort_nth_code
+   is \<open>uncurry insert_sort_nth\<close>
+   :: \<open>[\<lambda>(vm, remove). (\<forall>x\<in>#mset remove. x < length (fst vm))]\<^sub>a
+      vmtf_conc\<^sup>k *\<^sub>a (arl_assn uint32_nat_assn)\<^sup>d  \<rightarrow>
+       arl_assn uint32_nat_assn\<close>
+  unfolding insert_sort_nth_def insert_sort_def insert_sort_inner_nth_def[symmetric]
+  supply [[goals_limit = 1]]
+  supply mset_eq_setD[dest] mset_eq_length[dest]
+  by sepref
+
+declare insert_sort_nth_code.refine[sepref_fr_rules]
+
+sepref_definition vmtf_en_dequeue_code
+   is \<open>uncurry (RETURN oo vmtf_en_dequeue)\<close>
+   :: \<open>[\<lambda>(L,(A,m,lst,next_search)). L < length A \<and> (lst \<noteq> None \<longrightarrow> the lst < length A) \<and>
+        vmtf_dequeue_pre (L,A)]\<^sub>a
+        uint32_nat_assn\<^sup>k *\<^sub>a vmtf_conc\<^sup>d \<rightarrow> vmtf_conc\<close>
+  supply [[goals_limit = 1]]
+  supply vmtf_dequeue_def[simp] if_splits[split] vmtf_dequeue_pre_def[simp]
+  unfolding vmtf_en_dequeue_def
+  by sepref
+
+declare vmtf_en_dequeue_code.refine[sepref_fr_rules]
+
+lemma (in -) id_ref: \<open>(return o id, RETURN o id) \<in> R\<^sup>d \<rightarrow>\<^sub>a R\<close>
+  by sepref_to_hoare sep_auto
+
+lemma insert_sort_nth_reorder:
+   \<open>(uncurry insert_sort_nth, uncurry reorder_remove) \<in>
+      Id \<times>\<^sub>r \<langle>Id\<rangle>list_rel \<rightarrow>\<^sub>f \<langle>Id\<rangle> nres_rel\<close>
+  using insert_sort_reorder_remove[unfolded fref_def nres_rel_def]
+  by (intro frefI nres_relI) (fastforce simp: insert_sort_nth_def)
+
+lemma (in -) insert_sort_nth_code_reorder_remove[sepref_fr_rules]:
+   \<open>(uncurry insert_sort_nth_code, uncurry reorder_remove) \<in>
+      [\<lambda>((a, _), b). \<forall>x\<in>set b. x < length a]\<^sub>a
+      vmtf_conc\<^sup>k *\<^sub>a (arl_assn uint32_nat_assn)\<^sup>d \<rightarrow> arl_assn uint32_nat_assn\<close>
+  using insert_sort_nth_code.refine[FCOMP insert_sort_nth_reorder]
+  by auto
+
+context twl_array_code_ops
+begin
+
+sepref_thm vmtf_flush_code
+   is \<open>vmtf_flush\<close>
+   :: \<open>[\<lambda>a. \<exists>M. a \<in> vmtf_imp M]\<^sub>a vmtf_remove_conc\<^sup>d \<rightarrow> vmtf_remove_conc\<close>
+  supply [[goals_limit = 1]]
+  supply vmtf_en_dequeue_pre_def[simp] vmtf_imp_insert_sort_nth_code_preD[dest]
+  unfolding vmtf_flush_def
+  apply (rewrite
+        at \<open>[]\<close> in \<open>\<lambda>(_, removed). do {removed' \<leftarrow> _; (vm, _) \<leftarrow> _; RETURN (_, \<hole>)}\<close>
+        to \<open>emptied_list removed'\<close>
+          emptied_list_def[symmetric]
+     )
+  by sepref
+
+
+concrete_definition (in -) vmtf_flush_code
+   uses twl_array_code_ops.vmtf_flush_code.refine_raw
+   is \<open>(?f,_)\<in>_\<close>
+
+prepare_code_thms (in -) vmtf_flush_code_def
+
+lemmas trail_dump_code_refine[sepref_fr_rules] =
+   vmtf_flush_code.refine[of \<A>\<^sub>i\<^sub>n]
+
+declare vmtf_flush_code.refine[sepref_fr_rules]
+
+sepref_thm vmtf_dump_and_unset_code
+  is \<open>uncurry (RETURN oo vmtf_dump_and_unset)\<close>
+  :: \<open>[\<lambda>(L, ((A, m, lst, next_search), _)).
+      L < length A \<and> (next_search \<noteq> None \<longrightarrow> the next_search < length A)]\<^sub>a
+      uint32_nat_assn\<^sup>k *\<^sub>a vmtf_remove_conc\<^sup>d \<rightarrow> vmtf_remove_conc\<close>
+  supply image_image[simp] uminus_\<A>\<^sub>i\<^sub>n_iff[iff] in_diffD[dest] option.splits[split]
+  supply [[goals_limit=1]]
+  unfolding  vmtf_dump_and_unset_def vmtf_dump_def
+   vmtf_unset_def save_phase_def
+  apply (rewrite in \<open>If (_ \<or> _)\<close> short_circuit_conv)
+  by sepref
+
+concrete_definition (in -) vmtf_dump_and_unset_code
+  uses twl_array_code_ops.vmtf_dump_and_unset_code.refine_raw
+  is \<open>(uncurry ?f,_)\<in>_\<close>
+
+prepare_code_thms (in -) vmtf_dump_and_unset_code_def
+
+lemmas vmtf_dump_and_unset_hnr[sepref_fr_rules] =
+   vmtf_dump_and_unset_code.refine
+
+sepref_thm vmtf_unset_code
+  is \<open>uncurry (RETURN oo vmtf_unset)\<close>
+  :: \<open>[\<lambda>(L, vm). \<exists>M. L = atm_of(lit_of (hd M)) \<and> vm \<in> vmtf_imp M \<and> M \<noteq> [] \<and>
+          literals_are_in_\<L>\<^sub>i\<^sub>n (lit_of `# mset M)]\<^sub>a
+     uint32_nat_assn\<^sup>k *\<^sub>a vmtf_remove_conc\<^sup>d \<rightarrow> vmtf_remove_conc\<close>
+  supply [[goals_limit=1]] option.splits[split] vmtf_imp_def[simp] in_\<L>\<^sub>a\<^sub>l\<^sub>l_atm_of_in_atms_of_iff[simp]
+    neq_NilE[elim!] literals_are_in_\<L>\<^sub>i\<^sub>n_add_mset[simp]
+  unfolding vmtf_unset_def
+  apply (rewrite in \<open>If (_ \<or> _)\<close> short_circuit_conv)
+  by sepref
+
+concrete_definition (in -) vmtf_unset_code
+   uses twl_array_code_ops.vmtf_unset_code.refine_raw
+   is \<open>(uncurry ?f, _) \<in> _\<close>
+
+prepare_code_thms (in -) vmtf_unset_code_def
+
+lemmas vmtf_unset_code_code[sepref_fr_rules] =
+   vmtf_unset_code.refine[of \<A>\<^sub>i\<^sub>n]
+
+end
 end
