Weidenbach_Book/CDCL_Two_Watched_Literals_List_Watched_Domain.thy
@@ -247,6 +247,9 @@ qed
 lemma in_\<L>\<^sub>a\<^sub>l\<^sub>l_atm_of_in_atms_of_iff: \<open>x \<in># \<L>\<^sub>a\<^sub>l\<^sub>l \<longleftrightarrow> atm_of x \<in> atms_of \<L>\<^sub>a\<^sub>l\<^sub>l\<close>
   by (cases x) (auto simp: \<L>\<^sub>a\<^sub>l\<^sub>l_def atms_of_def atm_of_eq_atm_of image_Un image_image)
 
+lemma uminus_\<A>\<^sub>i\<^sub>n_iff: \<open>- L \<in># \<L>\<^sub>a\<^sub>l\<^sub>l \<longleftrightarrow> L \<in># \<L>\<^sub>a\<^sub>l\<^sub>l\<close>
+  by (simp add: in_\<L>\<^sub>a\<^sub>l\<^sub>l_atm_of_in_atms_of_iff)
+
 definition literals_are_in_\<L>\<^sub>i\<^sub>n_mm :: \<open>nat clauses \<Rightarrow> bool\<close> where
   \<open>literals_are_in_\<L>\<^sub>i\<^sub>n_mm C \<longleftrightarrow> set_mset (all_lits_of_mm C) \<subseteq> set_mset \<L>\<^sub>a\<^sub>l\<^sub>l\<close>
 
